Frap/Exercises/Equiv.lean
@@ -5,7 +5,7 @@ open Com
 open CEval
 -- -- enable this if necessary
 -- attribute [local simp]
---   aeval beval insert' lookup' map_lookup_insert_eq map_lookup_insert_neq
+--   aeval beval empty update lookup_update_eq lookup_update_neq
 
 /-
 exercise (2-star)
