Frap/Exercises/Hoare.lean
@@ -15,17 +15,18 @@ attribute [local simp]
 exercise (2-star)
 
 The assignment rule looks backward to almost everyone the first time they see it.
-If it still seems puzzling to you, it may help to think a little about alternative "forward" rules. Here is a seemingly natural one:
+If it still seems puzzling to you, it may help to think a little about alternative "forward" rules.
+Here is a seemingly natural one:
   `{ True } x := a { x = a }`
 
-Give a counterexample showing that this rule is incorrect and use it to complete the proof belkow, showing that it is really a counterexample.
+Give a counterexample showing that this rule is incorrect and use it to complete the proof below, showing that it is really a counterexample.
 (Hint: The rule universally quantifies over the arithmetic expression `a`, and your counterexample needs to exhibit an `a` for which the rule doesn't work.)
 -/
 
 example : ∃ (a : AExp), ¬ (
     {* fun _ => True *}
-      <{ x := a }>
-    {* fun st => lookup' st x = aeval st a *}) := by
+      <{ x := <[a]> }>
+    {* fun st => st x = aeval st a *}) := by
   sorry
 
 /-
@@ -45,9 +46,9 @@ Prove that `swap` does what we expect.
 -/
 
 theorem swap_correct a₀ b₀ :
-    {* fun st => lookup' st x = a₀ ∧ lookup' st y = b₀ *}
+    {* fun st => st x = a₀ ∧ st y = b₀ *}
       swap_program
-    {* fun st => lookup' st x = b₀ ∧ lookup' st y = a₀ *} := by
+    {* fun st => st x = b₀ ∧ st y = a₀ *} := by
   sorry
 
 /-
@@ -56,7 +57,7 @@ Prove that `swap` satisfies the following specification.
 -/
 
 example :
-    {* fun st => lookup' st x ≤ lookup' st y *}
+    {* fun st => st x ≤ st y *}
       swap_program
-    {* fun st => lookup' st y ≤ lookup' st x *} := by
+    {* fun st => st y ≤ st x *} := by
   sorry
